some cleaning

trunk/color/Util/Nat/Log2.v
@@ -4,73 +4,74 @@ See the COPYRIGHTS and LICENSE files.
 
 - Leo Ducas, 2007-08-06
 
-log2
+Definition of log2 (floor) and exp2, and some equalities
 *)
-(**Definition of log2 (floor) and exp2, and some equalities *)
-
 
 Require Export Div2.
 Require Export Le.
+
 Lemma div2_le_n : forall n, div2 n <= n.
+
 Proof.
 cut (forall n, div2 n <= n /\ div2 (S n) <= S n).
 intros H n; generalize (H n); tauto.
-induction n;auto.
-inversion IHn; split;auto.
+induction n; auto.
+inversion IHn; split; auto.
 simpl. apply le_n_S. auto with arith.
 Qed.
 
 Inductive log2_prop : nat -> nat -> Prop :=
 | log2_prop_O : log2_prop 0 0
 | log2_prop_1 : log2_prop 1 0
-| log2_prop_p : forall p q, p <> 0 -> p <> 1 -> log2_prop (div2 p) q -> log2_prop p (S q).
+| log2_prop_p : forall p q,
+  p <> 0 -> p <> 1 -> log2_prop (div2 p) q -> log2_prop p (S q).
 
 Hint Constructors log2_prop.
 
-Fixpoint log2_aux (n count : nat) {struct count} : nat :=
-match count with
-| 0 => 0
-| S count' =>
-  match n with
+Fixpoint log2_aux n count {struct count} : nat :=
+  match count with
     | 0 => 0
-    | 1 => 0
-    | _ => S (log2_aux (div2 n) count')
-  end
-end.
+    | S count' =>
+      match n with
+        | 0 => 0
+        | 1 => 0
+        | _ => S (log2_aux (div2 n) count')
+      end
+  end.
 
 (* log2_aux is correct as soon as count >= n *)
 
 Lemma log2_aux_matches : forall count n, n <= count ->
   log2_prop n (log2_aux n count).
+
 Proof.
 induction count.
- intros.  assert (n = 0).   auto with arith.
- subst.  simpl.  auto. intros n Hn.
+ intros. assert (n = 0). auto with arith.
+ subst. simpl. auto. intros n Hn.
 destruct n.
- simpl;  auto.
+ simpl; auto.
 destruct n.
- simpl;  auto.
+ simpl; auto.
 simpl.
 apply log2_prop_p.
  intro; discriminate.
  intro H; discriminate.
 apply IHcount; eapply le_trans.
-apply le_n_S;apply div2_le_n.
+apply le_n_S; apply div2_le_n.
 apply le_S_n; assumption.
 Qed.
 
 Definition log2 n := log2_aux n n.
 
+Lemma log2_matches : forall n, log2_prop n (log2 n).
 
-Corollary log2_matches : forall n, log2_prop n (log2 n).
 Proof.
-unfold log2.
-intros.
-apply log2_aux_matches.
-auto with arith.
+unfold log2. intros. apply log2_aux_matches. auto with arith.
 Qed.
 
-Lemma log2_prop_func : forall p q, log2_prop p q -> forall q', log2_prop p q' -> q = q'.
+Lemma log2_prop_func : forall p q,
+  log2_prop p q -> forall q', log2_prop p q' -> q = q'.
+
 Proof.
 induction 1.
  inversion 1.
@@ -87,51 +88,55 @@ f_equal.
 eapply IHlog2_prop; eauto.
 Qed.
 
-Corollary log2_matches_log2_prop : forall n p, log2_prop n p -> p = log2 n.
-intros.
-eapply log2_prop_func.
- eassumption.
-apply log2_matches.
+Lemma log2_matches_log2_prop : forall n p, log2_prop n p -> p = log2 n.
+
+Proof.
+intros. eapply log2_prop_func. eassumption. apply log2_matches.
 Qed.
 
-Fixpoint exp2 n := match n with
-  |O => 1
-  |S i => 2* exp2 i
+Fixpoint exp2 n :=
+  match n with
+    | O => 1
+    | S i => 2 * exp2 i
   end.
 
 Require Export Omega.
 Require Export Even.
 
-Lemma double_div2 : forall n, S(2* (div2 n)) >= n.
-intro n.
-destruct (even_or_odd n).
-rewrite even_double;auto;unfold double;omega.
-rewrite odd_double;auto;unfold double;omega.
+Lemma double_div2 : forall n, S (2 * div2 n) >= n.
+
+Proof.
+intro n. destruct (even_or_odd n).
+rewrite even_double; auto; unfold double; omega.
+rewrite odd_double; auto; unfold double; omega.
 Qed.
 
 Lemma exp2_pos : forall n, exp2 n >0.
+
 Proof.
-intro;induction n;simpl;auto with *.
+intro; induction n; simpl; auto with *.
 Qed.
+
 Lemma exp2_log2_prop : forall n p, log2_prop n p -> exp2 (S p) > n.
+
 Proof.
 cut(forall n n' p, n'<=n -> log2_prop n' p -> exp2 (S p) > n').
 intros. eapply H. assert (n<=n). omega. eassumption. assumption.
-intro;induction n;intros. assert (n'=0). omega. subst. apply exp2_pos.
+intro; induction n; intros. assert (n'=0). omega. subst. apply exp2_pos.
 inversion H; auto.
-subst; inversion H0. simpl;auto.
+subst; inversion H0. simpl; auto.
 subst.
 assert (exp2 (S q) > div2 (S n)).
 apply IHn.
-simpl;destruct n;auto with *.
-assert (div2 n <= n);auto with *. apply div2_le_n.
+simpl; destruct n; auto with *.
+assert (div2 n <= n); auto with *. apply div2_le_n.
 assumption.
 change (2*exp2 (S q) > S n).
-generalize(double_div2 (S n));intro;omega.
+generalize(double_div2 (S n)); intro; omega.
 Qed.
 
-Theorem exp2_log2 : forall n, exp2(S (log2 n)) > n.
+Lemma exp2_log2 : forall n, exp2(S (log2 n)) > n.
+
 Proof.
-intro;apply exp2_log2_prop.
-apply log2_matches.
+intro; apply exp2_log2_prop. apply log2_matches.
 Qed.
